Juvix/Core/Main.lean
@@ -1,3 +1,4 @@
 
 import Juvix.Core.Main.Language
 import Juvix.Core.Main.Semantics
+import Juvix.Core.Main.Evaluator
